Output each property immediately instead of batching

examples/hwmcc_checker/translation/cake_tigerProgScript.sml
@@ -3,9 +3,10 @@
 *)
 Theory cake_tigerProg
 Ancestors
+  infer_cv  (* TODO Remove once we have a proper CF spec *)
   aig_cert_fullProg
 Libs
-  preamble ml_translatorLib basisFunctionsLib
+  cv_transLib preamble ml_translatorLib basisFunctionsLib
 
 val _ = translation_extends "aig_cert_fullProg";
 
@@ -38,16 +39,41 @@ Quote add_cakeml:
   case TextIO.inputAllFrom (Some fwitness) of
     None => TextIO.output TextIO.stdErr "cannot read witness file\n"
   | Some witness =>
-  case make_cert_strings model witness of
+  case (print "parsing..."; parse_and_process model witness) of
     Error (msg, _) => TextIO.output TextIO.stdErr msg
-  | Return certs => let
+  | Return
+      (mcirc, (mreset, (mnext, (mpreds, (mcnstrs, (mlive, (mlatches,
+        (wcirc, (wreset, (wnext, (wpreds, (wcnstrs, (wlive, (wlatches, interv)))))))))))))) =>
+    let
       fun write (name, cert) = let
         val oname =
           (case prefix of None => name | Some pfx => pfx ^ name) ^ ".cnf"
         val ostrm = TextIO.openOut oname
         val _     = TextIO.output ostrm cert
-        in TextIO.closeOut ostrm end
-      in List.app write certs end
+      in TextIO.closeOut ostrm end
+      val _ = print "parsing finished! continuing with encodings..."
+      val _ = write (
+        make_reset_string mcirc mreset mcnstrs mlatches wcirc wreset wcnstrs
+          wlatches)
+      val _ = write (
+        make_transition_string mcirc mnext mcnstrs mlatches wcirc wnext wcnstrs
+          wlatches)
+      val _ = write (
+        make_property_string mcirc mcnstrs mpreds wcirc wcnstrs wpreds)
+      val _ = write (
+        make_base_string wcirc wreset wcnstrs wpreds wlatches)
+      val _ = write (
+        make_step_string wcirc wnext wcnstrs wpreds wlatches)
+      val _ = write (
+        make_liveness_string mcirc mcnstrs mlive
+          wcirc wnext wcnstrs wpreds wlive wlatches interv)
+      val _ = write (
+        make_decrease_string wcirc wnext wcnstrs wpreds wlive wlatches interv)
+      val _ = write (
+        make_closure_string wcirc wnext wcnstrs wpreds wlive wlatches interv)
+      val _ = write (
+        make_consistent_string wcirc wnext wcnstrs wpreds wlive wlatches interv)
+    in () end
 End
 
 Quote add_cakeml:
@@ -76,3 +102,14 @@ val prog =
 Definition cake_tiger_prog_def:
   cake_tiger_prog = ^prog
 End
+
+(* TODO Remove once we have a proper CF spec *)
+(* for testing (type inference) ***********************************************)
+
+(*
+val _ = cv_auto_trans inferTheory.init_config_def;
+
+val _ = cv_trans_deep_embedding EVAL cake_tiger_prog_def;
+
+val basis_types = cv_eval “infertype_prog init_config cake_tiger_prog”;
+*)
