examples/hwmcc_checker/compilation/cake_tigerCompileScript.sml
@@ -3,9 +3,15 @@
 *)
 Theory cake_tigerCompile
 Ancestors
-  cake_tigerProg
+  cake_tigerProg x64_config
 Libs
   preamble eval_cake_compile_x64Lib
 
+Definition x64_config'_def:
+  x64_config' =
+  let x64_stack_conf = x64_backend_config.stack_conf with perf_calls := T in
+    x64_backend_config with stack_conf := x64_stack_conf
+End
+
 Theorem cake_tiger_compiled =
-  eval_cake_compile_x64 "" cake_tiger_prog_def "cake_tiger.S";
+  eval_cake_compile_x64_with_conf "" x64_config'_def cake_tiger_prog_def "cake_tiger.S";
