examples/hwmcc_checker/translation/aig_cert_fullProgScript.sml
@@ -12,9 +12,20 @@ val _ = translation_extends "aig_to_cnfProg";
 
 fun demonadify thm = SRULE [oneline bind_def, guard_def, UNCURRY] thm;
 
-val r = translate sptreeTheory.fromAList_def;
-val r = translate (aig_cert_fullTheory.make_cert_aig_def |> demonadify);
+val r = translate aig_cert_fullTheory.space_def;
+val r = translate aig_cert_fullTheory.clause_end_def;
 val r = translate aig_cert_fullTheory.lit_to_string_def;
 val r = translate aig_cert_fullTheory.clause_to_string_def;
 val r = translate aig_cert_fullTheory.cnf_to_string_def;
-val r = translate (aig_cert_fullTheory.make_cert_strings_def |> demonadify);
+
+val r = translate (aig_cert_fullTheory.parse_and_process_def |> demonadify);
+
+val r = translate aig_cert_fullTheory.make_reset_string_def;
+val r = translate aig_cert_fullTheory.make_transition_string_def;
+val r = translate aig_cert_fullTheory.make_property_string_def;
+val r = translate aig_cert_fullTheory.make_base_string_def;
+val r = translate aig_cert_fullTheory.make_step_string_def;
+val r = translate aig_cert_fullTheory.make_liveness_string_def;
+val r = translate aig_cert_fullTheory.make_decrease_string_def;
+val r = translate aig_cert_fullTheory.make_closure_string_def;
+val r = translate aig_cert_fullTheory.make_consistent_string_def;
